base/Control/Monad/Fail.v
@@ -34,14 +34,12 @@ Local Definition MonadFail__option_fail
 
 Program Instance MonadFail__option : MonadFail option :=
   fun _ k => k {| fail__ := fun {a} => MonadFail__option_fail |}.
-Admit Obligations.
 
 Local Definition MonadFail__list_fail : forall {a}, GHC.Base.String -> list a :=
   fun {a} => fun arg_0__ => nil.
 
 Program Instance MonadFail__list : MonadFail list :=
   fun _ k => k {| fail__ := fun {a} => MonadFail__list_fail |}.
-Admit Obligations.
 
 (* Skipping instance MonadFail__IO *)
 
