examples/containers/lib/Data/Set/Internal.v
@@ -950,7 +950,6 @@ Local Definition Semigroup__Set__op_zlzg__ {inst_a} `{GHC.Base.Ord inst_a}
 Program Instance Semigroup__Set_ {a} `{GHC.Base.Ord a}
    : Data.Semigroup.Semigroup (Set_ a) :=
   fun _ k => k {| Data.Semigroup.op_zlzg____ := Semigroup__Set__op_zlzg__ |}.
-Admit Obligations.
 
 Local Definition Monoid__Set__mappend {inst_a} `{GHC.Base.Ord inst_a}
    : (Set_ inst_a) -> (Set_ inst_a) -> (Set_ inst_a) :=
@@ -962,7 +961,6 @@ Program Instance Monoid__Set_ {a} `{GHC.Base.Ord a}
     k {| GHC.Base.mappend__ := Monoid__Set__mappend ;
          GHC.Base.mconcat__ := Monoid__Set__mconcat ;
          GHC.Base.mempty__ := Monoid__Set__mempty |}.
-Admit Obligations.
 
 Definition maxViewSure {a} : a -> Set_ a -> Set_ a -> prod a (Set_ a) :=
   let fix go arg_0__ arg_1__ arg_2__
@@ -1104,7 +1102,6 @@ Local Definition Semigroup__MergeSet_op_zlzg__ {inst_a}
 Program Instance Semigroup__MergeSet {a}
    : Data.Semigroup.Semigroup (MergeSet a) :=
   fun _ k => k {| Data.Semigroup.op_zlzg____ := Semigroup__MergeSet_op_zlzg__ |}.
-Admit Obligations.
 
 Local Definition Monoid__MergeSet_mappend {inst_a}
    : (MergeSet inst_a) -> (MergeSet inst_a) -> (MergeSet inst_a) :=
@@ -1119,7 +1116,6 @@ Program Instance Monoid__MergeSet {a} : GHC.Base.Monoid (MergeSet a) :=
     k {| GHC.Base.mappend__ := Monoid__MergeSet_mappend ;
          GHC.Base.mconcat__ := Monoid__MergeSet_mconcat ;
          GHC.Base.mempty__ := Monoid__MergeSet_mempty |}.
-Admit Obligations.
 
 Definition drop {a} : GHC.Num.Int -> Set_ a -> Set_ a :=
   fun arg_0__ arg_1__ =>
@@ -1241,7 +1237,6 @@ Program Instance Eq___Set_ {a} `{GHC.Base.Eq_ a} : GHC.Base.Eq_ (Set_ a) :=
   fun _ k =>
     k {| GHC.Base.op_zeze____ := Eq___Set__op_zeze__ ;
          GHC.Base.op_zsze____ := Eq___Set__op_zsze__ |}.
-Admit Obligations.
 
 Program Instance Ord__Set_ {a} `{GHC.Base.Ord a} : GHC.Base.Ord (Set_ a) :=
   fun _ k =>
@@ -1252,7 +1247,6 @@ Program Instance Ord__Set_ {a} `{GHC.Base.Ord a} : GHC.Base.Ord (Set_ a) :=
          GHC.Base.compare__ := Ord__Set__compare ;
          GHC.Base.max__ := Ord__Set__max ;
          GHC.Base.min__ := Ord__Set__min |}.
-Admit Obligations.
 
 Local Definition Foldable__Set__length : forall {a}, Set_ a -> GHC.Num.Int :=
   fun {a} => size.
@@ -1272,7 +1266,6 @@ Program Instance Foldable__Set_ : Data.Foldable.Foldable Set_ :=
          Data.Foldable.product__ := fun {a} `{GHC.Num.Num a} => Foldable__Set__product ;
          Data.Foldable.sum__ := fun {a} `{GHC.Num.Num a} => Foldable__Set__sum ;
          Data.Foldable.toList__ := fun {a} => Foldable__Set__toList |}.
-Admit Obligations.
 
 Module Notations.
 Notation "'_Data.Set.Internal.\\_'" := (op_zrzr__).
