examples/containers/lib/Extract.v
@@ -1,0 +1,1 @@
+../manual/Extract.v
